Valaig/Aig/Projections.lean
@@ -24,7 +24,11 @@ def step (aig : Aig) (state : Aig) (map : Array Lit) (var : Var)
     | .false         => (state, .false)
     | .input idx     => let state := state.addInput' idx
                         (state, idx.getLit state)
-    | .latch idx     => (state, mapLit (idx.getReset aig))
+    | .latch idx     =>
+      match _ : idx.getReset aig with
+      | none         => let state := state.addLatch' idx .false none
+                        (state, idx.getLit state)
+      | some reset   => (state, mapLit reset)
     | .and rhs0 rhs1 => state.addAnd (mapLit rhs0) (mapLit rhs1)
 
   (state, map.push lit)
@@ -35,13 +39,8 @@ variable {wf : aig.WellFormed}
 variable {swf : state.WellFormed}
 variable {valid : ∀ lit ∈ map, lit.validIn state}
 variable {size : var.idx = map.size}
-variable {idxInvalid : ∀ {idx}, aig[var] = .input idx → ¬idx.validIn state}
-
-@[simp, grind .]
-theorem Comb_step (comb : state.Comb) :
-    (step aig state map var).fst.Comb := by
-  unfold step
-  grind
+variable {inputInvalid : ∀ {idx}, aig[var] = .input idx → ¬idx.validIn state}
+variable {latchInvalid : ∀ {idx}, aig[var] = .latch idx → ¬idx.validIn state}
 
 @[simp, grind =]
 theorem size_step :
@@ -64,20 +63,27 @@ theorem inputs_not_validIn_step {idx : InputIdx} (valid : idx.validIn aig) (inva
   grind
 
 @[simp, grind .]
-theorem inputsInvalid_step {idx : InputIdx} (h : idx.validIn aig)
-    (hs : (idx.getVar aig < var ∧ idx.validIn state) ∨ idx.getVar aig = var) :
+theorem latch_validIn_step {idx : LatchIdx} (valid : idx.validIn aig)
+    (h : (idx.getVar aig < var ∧ idx.validIn state) ∨ (idx.getVar aig = var ∧ idx.getReset aig = none)) :
     idx.validIn (step aig state map var).fst := by
   unfold step
   grind
 
-include idxInvalid swf in
+@[simp, grind .]
+theorem latches_not_validIn_step {idx : LatchIdx} (valid : idx.validIn aig) (invalid : ¬idx.validIn state)
+    (gt : idx.getVar aig > var) :
+    ¬idx.validIn (step aig state map var).fst := by
+  unfold step
+  grind
+
+include inputInvalid latchInvalid swf in
 @[simp, grind .]
 theorem WellFormed_step :
     (step aig state map var).fst.WellFormed := by
   unfold step
   grind
 
-include idxInvalid in
+include inputInvalid in
 @[simp, grind .]
 theorem valid_step {lit : Lit}
    (h : lit ∈ (step aig state map var).snd) :
@@ -100,6 +106,8 @@ where
       (valid : ∀ lit ∈ map, lit.validIn state := by grind)
       (inputsInvalid : ∀ {var : Var} {idx h},
         aig[var]'h = .input idx -> var ≥ aig.iterVal it → ¬idx.validIn state := by grind)
+      (latchesInvalid : ∀ {var : Var} {idx h},
+        aig[var]'h = .latch idx -> var ≥ aig.iterVal it → ¬idx.validIn state := by grind)
       (size : (aig.iterVal it).idx = map.size := by grind) :=
     match it.step with
     | .done _ =>
@@ -110,21 +118,12 @@ where
   termination_by it.finitelyManySteps
 
 @[simp, grind .]
-theorem Comb_resetAig :
-    aig.resetAig.fst.Comb := by
-  grind [resetAig, @Comb_go]
-where
-  Comb_go {it state map swf inputsValid valid size} (comb : state.Comb) :
-      (resetAig.go aig wf it state map swf inputsValid valid size).fst.Comb := by
-    fun_induction resetAig.go <;> grind
-
-@[simp, grind .]
 theorem WellFormed_resetAig :
     aig.resetAig.fst.WellFormed := by
   grind [resetAig, @WellFormed_go]
 where
-  WellFormed_go {it state map swf inputsValid valid size} :
-      (resetAig.go aig wf it state map swf inputsValid valid size).fst.WellFormed := by
+  WellFormed_go {a b c d e f g h} :
+      (resetAig.go aig wf a b c d e f g h).fst.WellFormed := by
     fun_induction resetAig.go <;> grind
 
 @[simp, grind =]
@@ -132,8 +131,8 @@ theorem input_validIn_resetAig {idx : InputIdx} :
     idx.validIn aig.resetAig.fst ↔ idx.validIn aig := by
   grind [resetAig, @input_validIn_go]
 where
-  input_validIn_go {it state map swf inputsValid valid size} :
-      let res := resetAig.go aig wf it state map swf inputsValid valid size
+  input_validIn_go {it state a b c d e f} :
+      let res := resetAig.go aig wf it state a b c d e f
       idx.validIn res.fst ↔
       idx.validIn state ∨ ∃ h, idx.getVar aig h ≥ (aig.iterVal it) := by
     fun_induction resetAig.go <;> grind [resetAig.step]
@@ -148,30 +147,30 @@ theorem resetAig_validIn {lit : Lit.In aig} :
     (aig.resetAig.snd lit).validIn aig.resetAig.fst := by
   grind [resetAig, @go_validIn]
 where
-  go_validIn {it state map swf inputsValid valid size} :
-      let res := resetAig.go aig wf it state map swf inputsValid valid size
+  go_validIn {a b c d e f g h} :
+      let res := resetAig.go aig wf a b c d e f g h
       (res.snd lit).validIn res.fst := by
     fun_induction resetAig.go <;> grind
 
 section denote_resetAig
 
 variable {state : Aig} {map : Array Lit} {swf : state.WellFormed}
-variable {denote : ∀ {var : Var} (lt : var.idx < map.size), state.denote map[var.idx] 0 assign = aig.denoteVar var 0 assign}
+variable {denote : ∀ {assign} {var : Var} (lt : var.idx < map.size),
+           state.denoteComb map[var.idx] assign = aig.denoteResetVar var assign}
 
 include denote in
-@[local grind .]
 theorem denote_mapTo (lit : Lit) {lt : lit.var.idx < map.size} :
-      state.denote (lit.mapTo map[lit.var.idx]) 0 assign swf = aig.denote lit 0 assign wf := by
-    simp only [Lit.mapTo_eq, denote_eq, lt, ←denote]
-    grind
+      state.denoteComb (lit.mapTo map[lit.var.idx]) assign swf = aig.denoteReset lit assign wf := by
+    grind [denoteReset_eq_denoteResetVar]
 
 include denote in
 @[local grind =]
-theorem denote_step {var var' inputsValid valid size}
-    {idxInvalid : ∀ {idx}, aig[var'] = .input idx → ¬idx.validIn state} :
-    let res := resetAig.step aig state map var' valid wf inputsValid size
+theorem denote_step {var var' a b c}
+    {inputInvalid : ∀ {idx}, aig[var'] = .input idx → ¬idx.validIn state}
+    {latchInvalid : ∀ {idx}, aig[var'] = .latch idx → ¬idx.validIn state} :
+    let res := resetAig.step aig state map var' a wf b c
     (lt : var.idx < res.snd.size) →
-      res.fst.denote res.snd[var.idx] 0 assign = aig.denoteVar var 0 assign := by
+      res.fst.denoteComb res.snd[var.idx] assign = aig.denoteResetVar var assign := by
   intro res h
   rw [show res.snd[var.idx] = (map.push res.snd[map.size])[var.idx] by simp [res, resetAig.step], Array.getElem_push]
   split
@@ -180,12 +179,15 @@ theorem denote_step {var var' inputsValid valid size}
   · have : var = var' := by grind
     cases h : aig[var']
     <;> simp only [res, resetAig.step, Array.getElem_push_eq]
-    <;> grind -splitMatch -splitIte
+    · grind -splitMatch -splitIte
+    · grind -splitMatch -splitIte
+    · grind -splitIte [denote_mapTo (aig := aig)]
+    · grind -splitMatch -splitIte [denote_mapTo (aig := aig)]
 
 include denote in
-theorem denote_go (lit : Lit.In aig) {it inputsValid valid size wf'} :
-    let res := resetAig.go aig wf it state map swf inputsValid valid size
-    res.fst.denote (res.snd lit) 0 assign wf' = aig.denote lit 0 assign := by
+theorem denote_go (lit : Lit.In aig) {it a b c d wf'} :
+    let res := resetAig.go aig wf it state map swf a b c d
+    res.fst.denoteComb (res.snd lit) assign wf' = aig.denoteReset lit assign := by
   fun_induction resetAig.go
   · grind only [denote_mapTo]
   next ih =>
@@ -197,6 +199,6 @@ end denote_resetAig
 
 @[simp, grind =]
 theorem denote_resetAig {assign} {lit : Lit.In aig} :
-    aig.resetAig.fst.denote (aig.resetAig.snd lit) 0 assign =
-    aig.denote lit 0 assign wf := by
+    aig.resetAig.fst.denoteComb (aig.resetAig.snd lit) assign =
+    aig.denoteReset lit assign wf := by
   grind [resetAig, denote_go]
